



Simplify Boolean expression 8

Simplify this Boolean expression:

$$(A \vee B) \wedge (B \vee B) \wedge (B \vee A)$$

The expression simplifies to:

- ☐ True (1)
- ☐ False (0)
- ☐ A
- ☐ B

All teaching materials on this site are available under a CC BY-NC-SA 4.0 license, except where otherwise stated.





Simplify Boolean expression 9

Using the laws of Boolean algebra, simplify this Boolean expression:

$$B \wedge (A \vee A) \vee B \wedge \neg A$$

The expression simplifies to:

- ☐ B
- ☐ True (1)
- ☐ A
- ☐ False (0)

Quiz:

STEM SMART Computer Science Week 31

All teaching materials on this site are available under a CC BY-NC-SA 4.0 license, except where otherwise stated.





Simplify Boolean expression 7

Use the laws of Boolean algebra to simplify the Boolean expression below.

$$(B \vee \neg B) \wedge (B \vee A)$$

Which of the following options shows the simplest equivalent logic?

- ☐ 0
- ☐ 1
- ☐ $B \vee A$
- ☐ $B \vee \neg B \wedge A$

Quiz:

[STEM SMART Computer Science Week 31](#)

All teaching materials on this site are available under a [CC BY-NC-SA 4.0](#) license, except where otherwise stated.





Simplify Boolean expression 3

Use the Boolean identities to simplify the Boolean expression below.

$$A \vee (B \wedge 1)$$

Which of the following options shows the simplest equivalent logic?

- ☐ A
- ☐ 0
- ☐ $A \vee B$
- ☐ $A \wedge B$
- ☐ B
- ☐ 1

Quiz:

STEM SMART Computer Science Week 31

All teaching materials on this site are available under a CC BY-NC-SA 4.0 license, except where otherwise stated.





Simplify Boolean expression 5

Use the laws of Boolean algebra to simplify the Boolean expression below.

$$B \vee \neg B \wedge A$$

Which of the following options shows the simplest equivalent logic?

- ☐ $A \vee B$
- ☐ $\neg B \vee A$
- ☐ A
- ☐ B

Quiz:

[STEM SMART Computer Science Week 31](#)

All teaching materials on this site are available under a CC BY-NC-SA 4.0 license, except where otherwise stated.





Simplify Boolean expression 6

Use the laws of Boolean algebra to simplify the Boolean expression below.

$$(A \wedge \neg B) \vee (A \wedge B)$$

Which of the following options shows the simplest equivalent logic?

- ☐ 1
- ☐ $A \wedge (B \vee \neg B)$
- ☐ $A \wedge B$
- ☐ A

Quiz:

STEM SMART Computer Science Week 31

All teaching materials on this site are available under a CC BY-NC-SA 4.0 license, except where otherwise stated.





Simplify Boolean expression 1

Use the Boolean identities to simplify the Boolean expression below.

$$X \wedge (Y \vee 1)$$

Which of the following options shows the simplest equivalent logic?

- ☐ Y
- ☐ 1
- ☐ 0
- ☐ X
- ☐ $X \wedge Y$
- ☐ $X \vee Y$

Quiz:

STEM SMART Computer Science Week 31

All teaching materials on this site are available under a CC BY-NC-SA 4.0 license, except where otherwise stated.





Boolean identities and laws 1

Boolean expressions can be manipulated using basic Boolean identities and laws. A Boolean identity is a statement of equivalence where the expression on the left of the equals sign has the same logic as the expression on the right.

Which of the following identities is **not** True?

- ☐ $A \vee 0 = A$
- ☐ $A \wedge \neg A = 0$
- ☐ $A \vee \neg A = 1$
- ☐ $A \wedge \neg A = 1$

Quiz:

STEM SMART Computer Science Week 31

All teaching materials on this site are available under a CC BY-NC-SA 4.0 license, except where otherwise stated.





Simplify Boolean expression 11

Using the laws of Boolean algebra, simplify this Boolean expression:

$$\neg(\neg(A \wedge B)) \vee A \vee B \vee C$$

The expression simplifies to:

- ☐ $A \vee B \vee C$
- ☐ $(A \wedge B) \vee C$
- ☐ False (0)
- ☐ $\neg C$

Quiz:

[STEM SMART Computer Science Week 31](#)

All teaching materials on this site are available under a CC BY-NC-SA 4.0 license, except where otherwise stated.





Simplify Boolean expression 13

There is more than one way to make use of the laws of Boolean algebra to simplify the expression below:

$$(A \vee B) \wedge (B \vee C \wedge (D \vee \neg D))$$

One option is:

$$(A \vee B) \wedge (B \vee C \wedge (D \vee \neg D))$$

$$= (A \vee B) \wedge (B \vee C \wedge 1)$$

$$= (A \vee B) \wedge (B \vee C)$$

$$= B \vee (A \wedge C)$$

Select a method from the options below that will also simplify the Boolean expression given above:

$$(A \vee B) \wedge (B \vee C \wedge (D \vee \neg D))$$

$$= (A \vee B) \wedge (B \vee C \wedge 1)$$

$$= (A \vee B) \wedge (B \vee C)$$

$$= (A \wedge B) \vee (A \wedge C) \vee (B \wedge B) \vee (B \wedge C)$$



$$= (A \wedge B) \vee (A \wedge C) \vee B \vee (B \wedge C)$$

$$= (A \wedge B) \vee (A \wedge C) \vee B$$

$$= B \vee (A \wedge B) \vee (A \wedge C)$$

$$= B \vee (A \wedge C)$$

$$(A \vee B) \wedge (B \vee C \wedge (D \vee \neg D))$$

$$= (A \vee B) \wedge (B \vee C \wedge 1)$$

$$= (A \vee B) \wedge (B \vee C)$$

$$= (A \vee B) \wedge (A \vee C) \wedge (B \vee B) \wedge (B \vee C)$$



$$= (A \vee B) \wedge (A \vee C) \wedge 1 \wedge (B \vee C)$$

$$= (A \vee B) \wedge (A \vee C) \wedge (B \vee C)$$

$$= B \vee (A \vee C) \wedge (A \vee C)$$

$$= B \vee (A \wedge C)$$
